A12Kernel.lean
@@ -254,6 +254,7 @@ import A12Kernel.Elaboration.StringToNumberComputationRun
 import A12Kernel.Elaboration.ScalarComputationRun
 import A12Kernel.Elaboration.ScalarComputationRunRelation
 import A12Kernel.Elaboration.ScalarComputationRunResult
+import A12Kernel.Elaboration.ScalarComputationFormalInput
 import A12Kernel.Elaboration.EnumerationComputation
 import A12Kernel.Elaboration.EnumerationComputationResult
 import A12Kernel.Elaboration.AddressedEnumerationComputation
